progress on proofmode

veric/proofmode.v
@@ -1,7 +1,7 @@
 From iris.proofmode Require Import coq_tactics reduction spec_patterns.
 From iris.proofmode Require Export tactics.
-Require Import VST.veric.Clight_core.
-Require Import VST.veric.lifting.
+From compcert.common Require Import Values.
+From VST.veric Require Import mpred juicy_base Clight_base Clight_core mapsto_memory_block lifting_expr lifting.
 
 Notation envs_entails := (envs_entails(PROP := monpred.monPredI _ _)).
 
@@ -21,8 +21,34 @@ Tactic Notation "wp_expr_eval" tactic3(t) :=
   end.
 Ltac wp_expr_simpl := wp_expr_eval simpl.
 
-Definition PureExec ge φ (n : nat) s1 s2 := φ →
-  forall f k ve te m, step ge (State f s1 k ve te) m (State f s2 k ve te) m.
+Inductive pure_step_n ge : nat -> Clight.statement -> Clight.statement -> Prop :=
+| pure_step_0 : forall s, pure_step_n ge O s s
+| pure_step_step : forall s1 s2 s3 n (Hstep : forall f k ve te m, step ge (State f s1 k ve te) m (State f s2 k ve te) m)
+    (Hsteps : pure_step_n ge n s2 s3), pure_step_n ge (S n) s1 s3.
+
+Definition PureExec ge φ (n : nat) s1 s2 : Prop := φ → pure_step_n ge n s1 s2.
+
+Lemma wp_pure_step_later `{!VSTGS OK_ty Σ} OK_spec ge E f s1 s2 φ n Q :
+  PureExec ge φ n s1 s2 →
+  φ →
+  (bi_laterN(PROP := monpred.monPredI _ _) n (wp OK_spec ge E f s2 Q) ⊢ wp OK_spec ge E f s1 Q).
+Proof.
+  intros Hexec ?; induction Hexec; [done | | done].
+  rewrite /= IHp /wp.
+  iIntros "H" (???) "L Hk".
+  rewrite /assert_safe /=.
+  do 4 (iApply embed_forall; iIntros (?)).
+  iIntros "Hρ %%".
+  iApply juicy_extspec.jsafe_local_step.
+  { apply Hstep. }
+  iSpecialize ("H" with "[//]").
+  rewrite !bi.later_wand.
+  iSpecialize ("H" with "L Hk").
+  iPoseProof (embed_later with "H") as "H".
+  iApply ("H" with "[Hρ]"); try done.
+  rewrite embed_later; iIntros "!>".
+  iApply "Hρ".
+Qed.
 
 Lemma tac_wp_pure `{!VSTGS OK_ty Σ} Δ Δ' OK_spec ge E f e1 e2 φ n Q :
   PureExec ge φ n e1 e2 →
@@ -32,17 +58,18 @@ Lemma tac_wp_pure `{!VSTGS OK_ty Σ} Δ Δ' OK_spec ge E f e1 e2 φ n Q :
   envs_entails Δ (wp OK_spec ge E f e1 Q).
 Proof.
   rewrite envs_entails_unseal=> ??? HΔ'. rewrite into_laterN_env_sound /=.
-  (* We want [pure_exec_fill] to be available to TC search locally. *)
-  pose proof @pure_exec_fill.
-  rewrite HΔ' -lifting.wp_pure_step_later //.
-  iIntros "Hwp !> _" => //.
+  rewrite HΔ'. etrans; last by eapply wp_pure_step_later.
+  iIntros "Hwp !>"; iApply "Hwp".
 Qed.
 
-Lemma tac_wp_load Δ Δ' s E i K b l q v Φ :
+(* Not sure how this will work, since we can't have pointer values as literals in
+   our program syntax. *)
+Lemma tac_wp_load `{!VSTGS OK_ty Σ} Δ Δ' ge E f i e b q t v (Q : val → assert) :
   MaybeIntoLaterNEnvs 1 Δ Δ' →
-  envs_lookup i Δ' = Some (b, l ↦{q} v)%I →
-  envs_entails Δ' (WP fill K (Val v) @ s; E {{ Φ }}) →
-  envs_entails Δ (WP fill K (Load (LitV l)) @ s; E {{ Φ }}).
+  envs_entails Δ' (wp_lvalue ge E f e (λ '(bl, o),
+    <affine> ⌜envs_lookup i Δ' = Some (b, ⎡mapsto q t (Vptr bl (Ptrofs.repr o)) v⎤)⌝ ∗
+    Q v))%I →
+  envs_entails Δ (wp_expr ge E f e Q).
 Proof.
   rewrite envs_entails_unseal=> ?? Hi.
   rewrite -wp_bind. eapply wand_apply; first by apply wand_entails, wp_load.
